Start moving Constructor from Point- to Code-based

src/Constructor.v
@@ -1,12 +1,9 @@
 (** * A constructor for simple types *)
 
-Require Export Points.
-(*
-Require Import BohmTrees.
-*)
+Require Export Codes.
+Open Scope code_scope.
 
 Section Exp.
-  Open Scope code_scope.
   Variable Var : Set.
   Let a := make_var Var 0.
   Let b := make_var Var 1.
@@ -14,15 +11,15 @@ Section Exp.
   Definition Exp := Eval compute in close (\a, \b, \f, b o f o a).
 End Exp.
 Notation "x --> y" := (Exp _ * x * y)%code : code_scope.
-Notation "x --> y" := ([Exp _] * x * y)%point : point_scope.
 
-Lemma exp_i_i (Var : Set) : I --> I = (I : Point Var).
+Lemma exp_i_i (Var : Set) : I --> I = (I : Code Var).
 Proof.
+  (* TODO adapt the beta_eta tactic from Points to Codes:
   unfold Exp; beta_eta.
-Qed.
+  *)
+Admitted.
 
 Section Pair.
-  Open Scope code_scope.
   Variable Var : Set.
   Let x := make_var Var 0.
   Let y := make_var Var 1.
@@ -30,59 +27,93 @@ Section Pair.
   Definition Pair := Eval compute in close (\x,\y,\f, f * x * y).
 End Pair.
 Notation "<< x , y >>" := (Pair _ * x * y)%code : code_scope.
-Notation "<< x , y >>" := ([Pair _] * x * y)%point : point_scope.
 
-Definition is_pair {Var : Set} (x : Point Var) := x = <<x * K, x * (K * I)>>.
-Lemma pair_is_pair (Var : Set) (x y : Point Var) : is_pair <<x, y>>.
+Definition is_pair {Var : Set} (x : Code Var) := x = <<x * K, x * (K * I)>>.
+Lemma pair_is_pair (Var : Set) (x y : Code Var) : is_pair <<x, y>>.
 Proof.
+  (* TODO adapt the beta_eta tactic from Points to Codes:
   hnf; unfold Pair; beta_reduce; auto.
-Qed.
+  *)
+Admitted.
 
-Definition sub_pair {Var : Set} (x : Point Var) := x [= <<TOP, TOP>>.
-Lemma sub_pair_pair (Var : Set) (x y : Point Var) : sub_pair <<x, y>>.
+Definition sub_pair {Var : Set} (x : Code Var) := x [= <<TOP, TOP>>.
+Lemma sub_pair_pair (Var : Set) (x y : Code Var) : sub_pair <<x, y>>.
 Proof.
+  (* TODO adapt the beta_eta tactic from Points to Codes:
   unfold sub_pair; unfold Pair; eta_expand as f; beta_reduce.
   monotonicity; auto.
-Qed.
+  *)
+Admitted.
 
-Definition sub_pair_elim_intro {Var : Set} (x : Point Var) :
+Definition sub_pair_elim_intro {Var : Set} (x : Code Var) :
   sub_pair x -> x [= <<x*K, x*(K*I)>>.
 Proof.
+  (* TODO adapt the beta_eta tactic from Points to Codes:
   unfold sub_pair; unfold Pair; simpl.
   intros H; eta_expand in H.
   eta_expand as f; beta_reduce.
-  (* TODO *)
+  TODO
+  *)
 Admitted.
-
-Definition A {Var : Set} :=
-  point_sup (<<s, r>> for s : Point Var for r : Point Var if r o s [= I).
-Notation "\\ x , y ; z" := (A * \x, \y, z)%code : code_scope.
-Notation "\\ x , y ; z" := (A * \x, \y, z)%point : point_scope.
-
-Section A_example.
-  Variable Var : Set.
-  Let a := [make_var Var 0].
-  Let a' := [make_var Var 1].
-  Let A_example : Point Var := point_close (\\a,a'; a --> a').
-End A_example.
 
 Section raise.
   Variable Var : Set.
-  Let x := [make_var Var 3].
-  Let y := [make_var Var 4].
+  Let x := make_var Var 3.
+  Let y := make_var Var 4.
 
-  Definition raise := point_close (\x, \y, x).
-  Definition lower := point_close (\x, x * TOP).
+  Definition raise := Eval compute in close (\x, \y, x).
+  Definition lower := Eval compute in close (\x, x * TOP).
 
-  Definition pull := point_close (\x, \y, x || [code_div] * y).
-  Definition push := point_close (\x, x * BOT).
+  Definition pull := Eval compute in close (\x, \y, x || code_div * y).
+  Definition push := Eval compute in close (\x, x * BOT).
 End raise.
 
-Lemma A_I_I (Var : Set) : <<I, I>> [= (A : Point Var).
+Section compose.
+  Variable Var : Set.
+  Let s := make_var Var 0.
+  Let a := make_var Var 1.
+  Let a' := make_var Var 2.
+  Let b := make_var Var 3.
+  Let b' := make_var Var 4.
+
+  (* TODO Get eta,I,K,B,C,S-abstraction working;
+     these are huge in I,K,S-abstraction. *)
+  Definition compose := Eval compute in close
+    (\s, s*\a,\a', s*\b,\b', <<a o b, b' o a'>>).
+
+  Definition conjugate := Eval compute in close
+    (\s, s*\a,\a', s*\b,\b', <<(a'-->b), (a-->b')>>).
+End compose.
+
+Definition A {Var : Set} : Code Var :=
+  Y * ( K * <<I, I>>
+     || K * <<raise _, lower _>>
+     || K * <<pull _, push _>>
+     || compose _
+     || conjugate _).
+
+Notation "\\ x , y ; z" := (A * \x, \y, z)%code : code_scope.
+
+Section A_example.
+  Variable Var : Set.
+  Let a := make_var Var 0.
+  Let a' := make_var Var 1.
+  Let A_example : Code Var := close (\\a,a'; a --> a').
+End A_example.
+
+(** ** A strong characterization of [A] *)
+
+Lemma A_pair (Var : Set) : (A : Code Var) [= <<TOP, TOP>>.
+Proof.
+  (* TODO *)
+Admitted.
+
+Lemma A_I_I (Var : Set) : <<I, I>> [= (A : Code Var).
 Proof.
   unfold A.
-  assert (I o I [= (I : Point Var)) as Heq; eta_expand; beta_reduce; auto.
-  (* TODO
+  (* TODO adapt the beta_eta tactic from Points to Codes:
+  assert (I o I [= (I : Code Var)) as Heq; eta_expand; beta_reduce; auto.
+  TODO
   apply Join_ub_eq with (i := restrict2_intro _ I I Heq).
   *)
 Admitted.
@@ -103,24 +134,7 @@ Proof.
   freeze div in (compute; eta_expand; beta_reduce).
   rewrite div_BOT; auto.
 Qed.
-*)
 
-Section compose.
-  Variable Var : Set.
-  Let s := [make_var Var 0].
-  Let a := [make_var Var 1].
-  Let a' := [make_var Var 2].
-  Let b := [make_var Var 3].
-  Let b' := [make_var Var 4].
-
-  Definition compose := point_close
-    (\s, s*\a,\a', s*\b,\b', <<a o b, b' o a'>>).
-
-  Definition conjugate := point_close
-    (\s, s*\a,\a', s*\b,\b', <<(a'-->b), (a-->b')>>).
-End compose.
-
-(*
 Lemma A_compose : forall a, A_prop a -> A_prop (compose * a).
 Proof.
   intros a H.
@@ -148,17 +162,10 @@ Proof.
 Qed.
 *)
 
-Definition A_def {Var : Set} : Point Var :=
-  Y * ( K * <<I, I>>
-     || K * <<raise _, lower _>>
-     || K * <<pull _, push _>>
-     || compose _
-     || conjugate _).
-
-Lemma A_sound (Var : Set) : A_def [= (A : Point Var).
+Lemma A_sound (Var : Set) (r s : Code Var) : <<s, r>> [= A -> r o s [= I.
 Proof.
-  (*
   unfold A.
+  (*
   apply Join_lub.
   *)
   (* unfold A_prop; split. *)
@@ -172,7 +179,7 @@ Proof.
   (* TODO *)
 Admitted.
 
-Lemma A_complete (Var : Set) : (A : Point Var) [= A_def.
+Lemma A_complete (Var : Set) (s r : Code Var) : r o s [= I -> <<s, r>> [= A.
 Proof.
   unfold A.
   (*
@@ -184,8 +191,3 @@ Proof.
   *)
   (* TODO *)
 Admitted.
-
-Theorem A_definable (Var : Set) : (A : Point Var) = A_def.
-Proof.
-  apply point_le_antisym ; apply A_sound || apply A_complete.
-Qed.
